Wiggle some more with balance_prop_inserted

examples/containers/theories/SetInductiveProofs.v
@@ -126,18 +126,17 @@ Proof. order_Bounds. Qed.
 
 (** The balancing property of a binary node *)
 Definition balance_prop sz1 sz2 :=
-  (sz1 + sz2 <= 1 \/ sz1 <= (delta * sz2) /\ sz2 <= delta * sz1)%Z.
+  (sz1 + sz2 <= 1 \/ sz1 <= delta * sz2 /\ sz2 <= delta * sz1)%Z.
 
 (** One precondition for [balanceL]: The left tree has been inserted to (but not by too much).
     This is mechanically derived from the context in the call to [balanceL] in [link], and
     unfortunately not very educational.
  *)
 Definition balance_prop_inserted sz1 sz2 :=
-  (delta * sz1 <= delta*delta*sz2 + delta*sz2 + delta + sz2 /\ sz2 <= delta * sz1)%Z.
+  (delta * sz1 <= delta*delta*sz2 + delta*sz2 + sz2 /\ sz2 <= sz1)%Z.
 
 (* NB: this does not work: 
-Definition balance_prop_inserted sz1 sz2 :=
-  (1 <= sz1)%Z  /\ balance_prop (sz1 - 1) sz2.
+Definition balance_prop_inserted sz1 sz2 := balance_prop sz1 sz2.
 *)
 
 Fixpoint sem (s : Set_ e) (i : e) : bool :=
@@ -681,8 +680,8 @@ Lemma balanceL_Desc:
     isLB lb x = true ->
     isUB ub x = true->
     balance_prop (size s1) (size s2) \/
-    balance_prop_inserted (size s1) (size s2) \/
-    balance_prop (size s1)%Z (size s2 + 1) ->
+    balance_prop_inserted (size s1 - 1) (size s2) /\ (1 <= size s1)%Z \/
+    balance_prop (size s1) (size s2 + 1) ->
     Desc (balanceL x s1 s2) lb ub (1 + size s1 + size s2) (fun i => sem s1 i || (i == x) || sem s2 i).
 Proof.
   intros.
@@ -707,7 +706,7 @@ Lemma balanceR_Desc:
     isLB lb x = true ->
     isUB ub x = true->
     balance_prop (size s1) (size s2) \/
-    balance_prop_inserted (size s2) (size s1) \/
+    balance_prop_inserted (size s2 - 1) (size s1) /\ (1 <= size s2)%Z  \/
     balance_prop (size s1 + 1) (size s2) ->
     Desc (balanceR x s1 s2) lb ub (1 + size s1 + size s2) (fun i => sem s1 i || (i == x) || sem s2 i).
 Proof.
